open import Algebra.Definitions
open import Data.Fin using (Fin)
open import Data.Product using (_,_; _Ã—_) renaming (projâ‚ to Ï€â‚; projâ‚‚ to Ï€â‚‚)
open import Data.Product.Relation.Binary.Pointwise.NonDependent using (Ã—-decSetoid)
open import Data.List using (List; filter; tabulate; []; _âˆ·_; _++_; map)
open import Data.List.Relation.Unary.Any using (here; there)
import Data.List.Membership.DecSetoid as Membership
open import Data.List.Membership.Setoid.Properties using (âˆˆ-resp-â‰ˆ)
import Data.List.Relation.Binary.Permutation.Setoid.Properties as PermutationProperties
open import Data.List.Relation.Binary.Pointwise using (Pointwise; []; _âˆ·_)
open import Data.Nat using (zero; suc; â„•; _*_; _+_)
open import Function using (_âˆ˜_)
open import Level using (_âŠ”_)
open import Relation.Nullary using (yes; no; Â¬_; Â¬?)
open import Relation.Nullary.Negation using (contradiction; contraposition)
open import Relation.Unary using (Pred; Decidable; _â‡’_)
open import Relation.Binary using (Setoid; DecSetoid; Rel; Reflexive; Symmetric; Transitive; _Respects_)
open import Relation.Binary.PropositionalEquality as PropositionalEq using (_â‰¡_; refl; cong)
import Relation.Binary.Reasoning.Setoid as EqReasoning

import RoutingLib.Data.List.Relation.Binary.Permutation.Setoid.Properties as PermutationPropertiesâ€²

open import RoutingLib.Iteration.Synchronous using (_^_)
open import RoutingLib.Routing.Algebra using (RawRoutingAlgebra; IsRoutingAlgebra)
open import RoutingLib.Routing.Prelude as Routing using () renaming (AdjacencyMatrix to AdjacencyMatrix')
import RoutingLib.Data.List.Relation.Binary.Permutation.Setoid.Properties as Perm
import RoutingLib.lmv34.Synchronous.Gamma_zero as Gamma_zero
import RoutingLib.lmv34.Synchronous.Gamma_zero.Algebra as Gamma_zero_Algebra
import RoutingLib.lmv34.Synchronous.Gamma_one as Gamma_one
import RoutingLib.lmv34.Synchronous.Gamma_one.Algebra as Gamma_one_Algebra
import RoutingLib.lmv34.Synchronous.Gamma_one.Properties as Gamma_one_Properties
import RoutingLib.lmv34.Synchronous.Gamma_two as Gamma_two
open import RoutingLib.lmv34.Synchronous.Gamma_two.Algebra as Gamma_two_Algebra using (IsComposition; RouteMapMatrix)
import RoutingLib.lmv34.Synchronous.Gamma_two.Properties as Gamma_two_Properties
import RoutingLib.lmv34.Synchronous.Gamma_three as Gamma_three
import RoutingLib.lmv34.Synchronous.Gamma_three.Algebra as Gamma_three_Algebra

module RoutingLib.lmv34.Synchronous.Gamma_three.Properties
  {a b â„“} {alg : RawRoutingAlgebra a b â„“}
  (isRAlg : IsRoutingAlgebra alg) {n}
  (A    : AdjacencyMatrix' alg n)
  (Imp Prot Exp : RouteMapMatrix isRAlg n )
  (A=Impâˆ˜Protâˆ˜Exp : IsComposition isRAlg n A Imp Prot Exp)
  where

open RawRoutingAlgebra alg
open Routing alg n renaming (I to M)
open Gamma_zero alg A
open Gamma_zero_Algebra alg n
open Gamma_one isRAlg A
open Gamma_one_Algebra isRAlg n
open Gamma_one_Properties isRAlg A
open Gamma_two isRAlg Imp Prot Exp
open Gamma_two_Algebra isRAlg n 
open Gamma_two_Properties isRAlg A Imp Prot Exp A=Impâˆ˜Protâˆ˜Exp
open Gamma_three isRAlg Imp Prot Exp
open Gamma_three_Algebra isRAlg n

open Membership Decğ”¸â‚› using (_âˆˆ?_; _âˆˆ_; _âˆ‰_; _âˆ‰?_)
open PermutationProperties ğ”¸â‚› using (filterâº; ++âº; ++-identityË¡; ++-identityÊ³; ++-assoc)
open PermutationPropertiesâ€² ğ”¸â‚› using (âˆ‰-resp-â†­)

------------------------------------
-- Î“â‚ƒ-State

infixr 4 _Ã—â‚›_
_Ã—â‚›_ : âˆ€ {â„“â‚ â„“â‚‚ â„“â‚ƒ â„“â‚„} â†’ DecSetoid â„“â‚ â„“â‚‚ â†’ DecSetoid â„“â‚ƒ â„“â‚„ â†’ DecSetoid _ _
_Ã—â‚›_ = Ã—-decSetoid

-- Î“â‚ƒ-State setoid
Î“â‚ƒ-State-decSetoid : DecSetoid _ _
Î“â‚ƒ-State-decSetoid = â‰ˆáµ¥-decSetoid Ã—â‚› â‰ˆáµ¥,â‚‚-decSetoid Ã—â‚› â‰ˆáµ¥,â‚‚-decSetoid Ã—â‚› â‰ˆáµ¥,â‚‚-decSetoid Ã—â‚› â‰ˆáµ¥,â‚‚-decSetoid

open DecSetoid Î“â‚ƒ-State-decSetoid using () renaming
  ( _â‰ˆ_    to _â‰ˆâ‚›_
  ; refl   to â‰ˆâ‚›-refl
  ; setoid to ğ•Šâ‚›
  )

open DecSetoid Î“â‚‚-State-decSetoid using () renaming
  ( _â‰ˆ_ to _â‰ˆâ‚›,â‚‚_)

------------------------------------
-- Operation properties

-- lmv34: Couldn't find bi-implication in the stdlib
infix 4 _â‡”_
_â‡”_ : âˆ€ {a â„“â‚ â„“â‚‚} {A : Set a} â†’ Pred A â„“â‚ â†’ Pred A â„“â‚‚ â†’ Pred A _
P â‡” Q = Î» x â†’ (P x â†’ Q x) Ã— (Q x â†’ P x)

filter-lemma : âˆ€ {p} {P P' : Pred Assignment p} (P? : Decidable P) (P?' : Decidable P')
               xs â†’ (âˆ€ x â†’ (P â‡” P') x) â†’ filter P? xs â†­ filter P?' xs
filter-lemma _ _ [] P=P' = â†­-refl
filter-lemma P? P?' (x âˆ· xs) P=P' with P? x | P?' x
... | yes _  | yes _    = â†­-prep x (filter-lemma P? P?' xs P=P')
... | yes Px | no Â¬P'x  = contradiction ((Ï€â‚ (P=P' x)) Px) Â¬P'x
... | no Â¬Px | yes P'x  = contradiction ((Ï€â‚‚ (P=P' x)) P'x) Â¬Px
... | no _   | no _     = filter-lemma P? P?' xs P=P'

minus-respects-â‰ˆâ‚ : âˆ€ {xs} â†’ (_âˆ‰ xs) Respects _â‰ˆâ‚_
minus-respects-â‰ˆâ‚ {(x âˆ· xs)} {y} {y'} y=y' Py with y' âˆˆ? (x âˆ· xs)
... | yes (here y'=x) = contradiction (here (â‰ˆâ‚-trans y=y' y'=x)) Py
... | yes (there Py') = contradiction (there (âˆˆ-resp-â‰ˆ ğ”¸â‚› (â‰ˆâ‚-sym y=y') Py')) Py
... | no Â¬Py' = Â¬Py'

minus-congâ‚— : LeftCongruent _â†­_ _-_
minus-congâ‚— {x = A} B=B' = filter-lemma (_âˆ‰? _) (_âˆ‰? _) A (Î» x â†’ âˆ‰-resp-â†­ B=B' , âˆ‰-resp-â†­ (â†­-sym B=B'))

minus-congáµ£ : RightCongruent _â†­_ _-_
minus-congáµ£ {x = A} A=A' = filterâº (Î» x â†’ Â¬? (x âˆˆ? A)) minus-respects-â‰ˆâ‚ A=A'

minus-cong : Congruentâ‚‚ _â†­_ _-_
minus-cong {A} {A'} {B} {B'} A=A' B=B' = begin
  A - B â†­âŸ¨ minus-congáµ£ {B} A=A' âŸ©
  A' - B â†­âŸ¨ minus-congâ‚— {A'} B=B' âŸ©
  A' - B' âˆ
  where open PermutationReasoning

minusáµ¥-cong : Congruentâ‚‚ _â‰ˆáµ¥,â‚‚_ _-áµ¥_
minusáµ¥-cong U=U' V=V' i j = minus-cong (U=U' i j) (V=V' i j)

minus-zeroâ‚— : LeftZero _â†­_ Ã˜ _-_
minus-zeroâ‚— xs = â†­-refl

minus-identityáµ£ : RightIdentity _â†­_ Ã˜ _-_
minus-identityáµ£ []       = â†­-refl
minus-identityáµ£ (x âˆ· xs) = â†­-prep x (minus-identityáµ£ xs)

âˆª-cong : Congruentâ‚‚ _â†­_ _âˆª_
âˆª-cong A=A' B=B' = PermutationProperties.++âº ğ”¸â‚› A=A' (minus-cong B=B' A=A')

âˆª-identityâ‚— : LeftIdentity _â†­_ Ã˜ _âˆª_
âˆª-identityâ‚— xs = minus-identityáµ£ xs

âˆª-identityáµ£ : RightIdentity _â†­_ Ã˜ _âˆª_
âˆª-identityáµ£ xs = ++-identityÊ³ xs

âˆªáµ¥-cong : Congruentâ‚‚ _â‰ˆáµ¥,â‚‚_ _âˆªáµ¥_
âˆªáµ¥-cong U=U' V=V' i j = âˆª-cong (U=U' i j) (V=V' i j)

diff-cong : âˆ€ {A A' B B'} â†’ A â†­ A' â†’ B â†­ B' â†’
            Ï€â‚ (diff A B) â†­ Ï€â‚ (diff A' B') Ã—
            Ï€â‚‚ (diff A B) â†­ Ï€â‚‚ (diff A' B')
diff-cong A=A' B=B' = minus-cong A=A' B=B' , minus-cong B=B' A=A'

diffáµ¥-cong : âˆ€ {U U' V V'} â†’ U â‰ˆáµ¥,â‚‚ U' â†’ V â‰ˆáµ¥,â‚‚ V' â†’
            Ï€â‚ (diffáµ¥ U V) â‰ˆáµ¥,â‚‚ Ï€â‚ (diffáµ¥ U' V') Ã—
            Ï€â‚‚ (diffáµ¥ U V) â‰ˆáµ¥,â‚‚ Ï€â‚‚ (diffáµ¥ U' V')
diffáµ¥-cong A=A' B=B' =
  (Î» i j â†’ minus-cong (A=A' i j) (B=B' i j)) ,
  (Î» i j â†’ minus-cong (B=B' i j) (A=A' i j))

Î“â‚ƒ,áµ¥-cong : âˆ€ {I I'} â†’ I â‰ˆáµ¥,â‚‚ I' â†’ Î“â‚ƒ,áµ¥ I â‰ˆáµ¥ Î“â‚ƒ,áµ¥ I'
Î“â‚ƒ,áµ¥-cong = Î“â‚‚,áµ¥-cong

Î“â‚ƒ,áµ¢-cong : âˆ€ {I I' âˆ‡ âˆ‡' Î” Î”'} â†’ I â‰ˆáµ¥,â‚‚ I' â†’ âˆ‡ â‰ˆáµ¥,â‚‚ âˆ‡' â†’ Î” â‰ˆáµ¥,â‚‚ Î”' â†’
            Î“â‚ƒ,áµ¢ I (âˆ‡ , Î”) â‰ˆáµ¥,â‚‚ Î“â‚ƒ,áµ¢ I' (âˆ‡' , Î”')
Î“â‚ƒ,áµ¢-cong I=I' âˆ‡=âˆ‡' Î”=Î”' = âˆªáµ¥-cong (minusáµ¥-cong I=I' (Î“â‚‚,áµ¢-cong âˆ‡=âˆ‡')) (Î“â‚‚,áµ¢-cong Î”=Î”')

Î“â‚ƒ,â‚’-cong : âˆ€ {V V'} â†’ V â‰ˆáµ¥ V' â†’ Î“â‚ƒ,â‚’ V â‰ˆáµ¥,â‚‚ Î“â‚ƒ,â‚’ V'
Î“â‚ƒ,â‚’-cong = Î“â‚‚,â‚’-cong

Î“â‚ƒ,â‚“-cong : âˆ€ {V V' O O'} â†’ V â‰ˆáµ¥ V' â†’ O â‰ˆáµ¥,â‚‚ O' â†’
            (Ï€â‚ (Î“â‚ƒ,â‚“ V O) â‰ˆáµ¥,â‚‚ Ï€â‚(Î“â‚ƒ,â‚“ V' O')) Ã—
            (Ï€â‚‚ (Î“â‚ƒ,â‚“ V O) â‰ˆáµ¥,â‚‚ Ï€â‚‚(Î“â‚ƒ,â‚“ V' O'))
Î“â‚ƒ,â‚“-cong V=V' O=O' = diffáµ¥-cong O=O' (Î“â‚ƒ,â‚’-cong V=V')

Î“â‚ƒ-cong : Congruentâ‚ _â‰ˆâ‚›_ Î“â‚ƒ
Î“â‚ƒ-cong (V=V' , I=I' , O=O' , âˆ‡=âˆ‡' , Î”=Î”') = 
  Î“â‚ƒ,áµ¥-cong I=I' ,
  Î“â‚ƒ,áµ¢-cong I=I' âˆ‡=âˆ‡' Î”=Î”' ,
  Î“â‚ƒ,â‚’-cong V=V' ,
  Ï€â‚ (Î“â‚ƒ,â‚“-cong V=V' O=O') ,
  Ï€â‚‚ (Î“â‚ƒ,â‚“-cong V=V' O=O')

------------------------------------
-- Theorems

-- diff-lemma is false as it is. Take for example A = {0, 0}, B = {0}.
-- What we need is:
  -- A and B have no duplicates.
postulate
  diff-lemma : âˆ€ A B â†’ let (âˆ‡ , Î”) = diff A B in
          (A - âˆ‡) âˆª Î” â†­ B

-- map-distrib is false as it is. Take for example f(x) = (0, âˆ), X = {(0,0)}, Y = {(0,âˆ)}.
-- What we need is:
  -- Y âŠ† X, and
  -- f is an injective function, or:
    -- f only acts on the second projection of the elements in X and Y (leaving the first unchanged), and
    -- X and Y have unique destinations (no two (d, s) and (d, s') with sâ‰ s').
postulate
  map-distrib : âˆ€ {f} X Y â†’ mapâ‚‚ f (X - Y) â†­ (mapâ‚‚ f X) - (mapâ‚‚ f Y)

âˆˆ-â€ -lemmaâ‚ : âˆ€ {X d v} â†’ (d , v) âˆˆ X â†’ Â¬(v â‰ˆ âˆ#) â†’ (d , v) âˆˆ X â€ 
âˆˆ-â€ -lemmaâ‚ {(d' , v') âˆ· X} (here (d=d' , v=v')) vâ‰ âˆ with v' â‰Ÿ âˆ#
... | yes v'=âˆ = contradiction (â‰ˆ-trans v=v' v'=âˆ) vâ‰ âˆ
... | no _     = here (d=d' , v=v')
âˆˆ-â€ -lemmaâ‚ {(d' , v') âˆ· X} (there dvâˆˆX) vâ‰ âˆ with v' â‰Ÿ âˆ#
... | yes v'=âˆ = âˆˆ-â€ -lemmaâ‚ dvâˆˆX vâ‰ âˆ
... | no _     = there (âˆˆ-â€ -lemmaâ‚ dvâˆˆX vâ‰ âˆ)

âˆˆ-â€ -lemmaâ‚‚ : âˆ€ {X d v} â†’ (d , v) âˆˆ X â€  â†’ (d , v) âˆˆ X
âˆˆ-â€ -lemmaâ‚‚ {((d' , v') âˆ· X)} dvâˆˆXâ€  with v' â‰Ÿ âˆ#
... | yes _ = there (âˆˆ-â€ -lemmaâ‚‚ {X} dvâˆˆXâ€ )
âˆˆ-â€ -lemmaâ‚‚ {(d' , v') âˆ· X} {d} {v} (here dv=dv') | no _ = here dv=dv'
âˆˆ-â€ -lemmaâ‚‚ {(d' , v') âˆ· X} {d} {v} (there dvâˆˆXâ€ ) | no _ = there (âˆˆ-â€ -lemmaâ‚‚ dvâˆˆXâ€ )

â€ -distrib : âˆ€ X Y â†’ (X - Y) â€  â†­ (X â€ ) - (Y â€ )
â€ -distrib [] Y = â†­-refl
â€ -distrib ((d , v) âˆ· X) Y with (d , v) âˆˆ? Y
... | yes dvâˆˆY = prf
  where prf : (X - Y) â€  â†­ (((d , v) âˆ· X) â€ ) - (Y â€ )
        prf with v â‰Ÿ âˆ#
        ... | yes _  = â€ -distrib X Y
        ... | no vâ‰ âˆ = prf'
          where prf' : (X - Y) â€  â†­ ((d , v) âˆ· (X â€ )) - (Y â€ )
                prf' with (d , v) âˆˆ? Y â€ 
                ... | yes _    = â€ -distrib X Y
                ... | no dvâˆ‰Yâ€  = contradiction (âˆˆ-â€ -lemmaâ‚ dvâˆˆY vâ‰ âˆ) dvâˆ‰Yâ€ 
... | no dvâˆ‰Y  = prf
  where prf : ((d , v) âˆ· (X - Y)) â€  â†­ ((d , v) âˆ· X) â€  - Y â€ 
        prf with v â‰Ÿ âˆ#
        ... | yes _ = â€ -distrib X Y
        ... | no _  = prf'
          where prf' : (d , v) âˆ· ((X - Y) â€ ) â†­ ((d , v) âˆ· (X â€ )) - Y â€ 
                prf' with (d , v) âˆˆ? Y â€ 
                ... | yes dvâˆˆYâ€  = contradiction dvâˆˆYâ€  (contraposition âˆˆ-â€ -lemmaâ‚‚ dvâˆ‰Y)
                ... | no _      = prep ((refl , â‰ˆ-refl)) (â€ -distrib X Y)

-- Lemma A.6
f-minus-distrib : âˆ€ f X Y  â†’ f [ X - Y ] â†­ f [ X ] - f [ Y ] 
f-minus-distrib f X Y = begin
                 f [ X - Y ]                     â‰¡âŸ¨âŸ©
                 (mapâ‚‚ f (X - Y)) â€               â†­âŸ¨ â€ -cong (map-distrib X Y) âŸ©
                 ((mapâ‚‚ f X) - (mapâ‚‚ f Y)) â€      â†­âŸ¨ â€ -distrib (mapâ‚‚ f X) (mapâ‚‚ f Y) âŸ©
                 ((mapâ‚‚ f X) â€ ) - ((mapâ‚‚ f Y) â€ ) â‰¡âŸ¨âŸ©
                 f [ X ] - f [ Y ] 
                 âˆ
                 where open PermutationReasoning

F-minus-distrib : âˆ€ F O O'  â†’ (F ã€– O -áµ¥ O' ã€—) â‰ˆáµ¥,â‚‚ ((F ã€– O  ã€—) -áµ¥ (F ã€– O' ã€—))
F-minus-distrib F O O' i j = f-minus-distrib (F i j) (O j i) (O' j i)

Î“â‚‚,áµ¢-distrib : âˆ€ O O' â†’ Î“â‚‚,áµ¢ (O -áµ¥ O') â‰ˆáµ¥,â‚‚ (Î“â‚‚,áµ¢ (O) -áµ¥ Î“â‚‚,áµ¢ (O'))
Î“â‚‚,áµ¢-distrib O O' i j = F-minus-distrib (Imp âˆ˜â‚˜ Prot) O O' i j

-- To show relationship of Î“â‚ƒ and Î“â‚‚ 
-- we simply need an invariant, so that we can equate each step of Î“â‚ƒ with a step of Î“â‚‚.
-- We only need to ensure that at each step the I component of Î“â‚ƒ is equal to the I component of Î“â‚‚.
-- Then the V, I, and O components will be the same at each step.

Î“â‚ƒ-invariant : Î“â‚ƒ-State â†’ Set (a âŠ” â„“)
Î“â‚ƒ-invariant (V , I , O , (âˆ‡ , Î”)) = Î“â‚‚,áµ¢ O â‰ˆáµ¥,â‚‚ Î“â‚ƒ,áµ¢ I  (âˆ‡ , Î”)

diffáµ¥-lemma : âˆ€ X Y â†’ let (âˆ‡ , Î”) = diffáµ¥ X Y in
              ((X -áµ¥ âˆ‡) âˆªáµ¥ Î”) â‰ˆáµ¥,â‚‚ Y
diffáµ¥-lemma X Y i j = diff-lemma (X i j) (Y i j)

Î“â‚ƒ-invariant-maintained : âˆ€ (S : Î“â‚ƒ-State) â†’ Î“â‚ƒ-invariant S â†’ Î“â‚ƒ-invariant (Î“â‚ƒ S) 
Î“â‚ƒ-invariant-maintained (V , I , O , (âˆ‡ , Î”)) inv = prf
   where
     prf : Î“â‚‚,áµ¢ (Î“â‚‚,â‚’ V) â‰ˆáµ¥,â‚‚ Î“â‚ƒ,áµ¢ (Î“â‚ƒ,áµ¢ I  (âˆ‡ , Î”))  (diffáµ¥ O (Î“â‚ƒ,â‚’ V))
     prf = begin
             Î“â‚‚,áµ¢ (Î“â‚‚,â‚’ V)                                                       â‰ˆâŸ¨ â‰ˆáµ¥,â‚‚-sym (diffáµ¥-lemma ((Î“â‚‚,áµ¢ O)) ((Î“â‚‚,áµ¢ (Î“â‚‚,â‚’ V)))) âŸ©
             ((Î“â‚‚,áµ¢ O) -áµ¥ (Î“â‚‚,áµ¢ (O) -áµ¥ Î“â‚‚,áµ¢ (Î“â‚‚,â‚’ V))) âˆªáµ¥ (Î“â‚‚,áµ¢ (Î“â‚‚,â‚’ V) -áµ¥ (Î“â‚‚,áµ¢ O)) â‰ˆâŸ¨ â‰ˆáµ¥,â‚‚-refl  âŸ©                    
             ((Î“â‚‚,áµ¢ O) -áµ¥ (Î“â‚‚,áµ¢ (O) -áµ¥ Î“â‚‚,áµ¢ (Î“â‚ƒ,â‚’ V))) âˆªáµ¥ (Î“â‚‚,áµ¢ (Î“â‚ƒ,â‚’ V) -áµ¥ (Î“â‚‚,áµ¢ O)) â‰ˆâŸ¨ âˆªáµ¥-cong {u = (Î“â‚‚,áµ¢ (Î“â‚ƒ,â‚’ V) -áµ¥ (Î“â‚‚,áµ¢ O))} ((minusáµ¥-cong {Î“â‚‚,áµ¢ O}  â‰ˆáµ¥,â‚‚-refl (â‰ˆáµ¥,â‚‚-sym (Î“â‚‚,áµ¢-distrib O (Î“â‚ƒ,â‚’ V))))) â‰ˆáµ¥,â‚‚-refl  âŸ©   
             ((Î“â‚‚,áµ¢ O) -áµ¥ (Î“â‚‚,áµ¢ (O -áµ¥ (Î“â‚ƒ,â‚’ V)))) âˆªáµ¥ (Î“â‚‚,áµ¢ (Î“â‚ƒ,â‚’ V) -áµ¥ (Î“â‚‚,áµ¢ O))     â‰ˆâŸ¨ âˆªáµ¥-cong â‰ˆáµ¥,â‚‚-refl ((â‰ˆáµ¥,â‚‚-sym ((Î“â‚‚,áµ¢-distrib (Î“â‚ƒ,â‚’ V) O))))  âŸ©
             ((Î“â‚‚,áµ¢ O) -áµ¥ (Î“â‚‚,áµ¢ (O -áµ¥ (Î“â‚ƒ,â‚’ V)))) âˆªáµ¥ (Î“â‚‚,áµ¢ ((Î“â‚ƒ,â‚’ V) -áµ¥ O)) â‰ˆâŸ¨ â‰ˆáµ¥,â‚‚-refl  âŸ©                                       
             Î“â‚ƒ,áµ¢ (Î“â‚‚,áµ¢ O)  (O -áµ¥ (Î“â‚ƒ,â‚’ V) , (Î“â‚ƒ,â‚’ V) -áµ¥ O)               â‰ˆâŸ¨ â‰ˆáµ¥,â‚‚-refl âŸ©                          
             Î“â‚ƒ,áµ¢ (Î“â‚‚,áµ¢ O)  (O -áµ¥ (Î“â‚ƒ,â‚’ V) , (Î“â‚ƒ,â‚’ V) -áµ¥ O)               â‰ˆâŸ¨ Î“â‚ƒ,áµ¢-cong {I = (Î“â‚‚,áµ¢ O)} {âˆ‡ = (O -áµ¥ (Î“â‚ƒ,â‚’ V))} {Î” = ((Î“â‚ƒ,â‚’ V) -áµ¥ O)}  inv â‰ˆáµ¥,â‚‚-refl â‰ˆáµ¥,â‚‚-refl  âŸ©
             Î“â‚ƒ,áµ¢ ((Î“â‚ƒ,áµ¢ I  (âˆ‡ , Î”)))  (O -áµ¥ (Î“â‚ƒ,â‚’ V) , (Î“â‚ƒ,â‚’ V) -áµ¥ O)   â‰ˆâŸ¨ â‰ˆáµ¥,â‚‚-refl âŸ©                                       
             Î“â‚ƒ,áµ¢ (Î“â‚ƒ,áµ¢ I  (âˆ‡ , Î”))  (diffáµ¥ O (Î“â‚ƒ,â‚’ V))
            âˆ
            where open EqReasoning ğ•â‚‚â‚›

Î“â‚ƒ-invariant-maintained-iter : âˆ€ (S : Î“â‚ƒ-State) k â†’ Î“â‚ƒ-invariant S â†’ Î“â‚ƒ-invariant ((Î“â‚ƒ ^ k) S) 
Î“â‚ƒ-invariant-maintained-iter S zero inv = inv 
Î“â‚ƒ-invariant-maintained-iter S (suc k) inv = Î“â‚ƒ-invariant-maintained ((Î“â‚ƒ ^ k) S) (Î“â‚ƒ-invariant-maintained-iter S k inv)  


Sâ‚ƒâ‰ˆSâ‚‚ : Î“â‚ƒ-State â†’ Î“â‚‚-State â†’ Set (a âŠ” â„“)
Sâ‚ƒâ‰ˆSâ‚‚ (V , I , O , (âˆ‡ , Î”)) (V' , I' , O') = (V , I , O) â‰ˆâ‚›,â‚‚ (V' , I' , O')

Sâ‚ƒâ‰ˆSâ‚‚-maintained : âˆ€ (S3 : Î“â‚ƒ-State) (S2 : Î“â‚‚-State) â†’ Sâ‚ƒâ‰ˆSâ‚‚ S3 S2 â†’ Î“â‚ƒ-invariant S3 â†’ Sâ‚ƒâ‰ˆSâ‚‚ (Î“â‚ƒ S3) (Î“â‚‚ S2)
Sâ‚ƒâ‰ˆSâ‚‚-maintained  (V , I , O , (âˆ‡ , Î”)) (V' , I' , O') ( Vâ‰ˆV' , (Iâ‰ˆI' , Oâ‰ˆO') ) inv = prfV , prfI , prfO
  where
    prfV : (Î“â‚ƒ,áµ¥ I) â‰ˆáµ¥ (Î“â‚‚,áµ¥ I')
    prfV = Î“â‚‚,áµ¥-cong Iâ‰ˆI'

    prfI : (Î“â‚ƒ,áµ¢ I (âˆ‡ , Î”)) â‰ˆáµ¥,â‚‚ (Î“â‚‚,áµ¢ O')
    prfI = begin
            Î“â‚ƒ,áµ¢ I (âˆ‡ , Î”)  â‰ˆâŸ¨ â‰ˆáµ¥,â‚‚-sym inv âŸ©             
            Î“â‚‚,áµ¢ O          â‰ˆâŸ¨ Î“â‚‚,áµ¢-cong Oâ‰ˆO' âŸ©             
            Î“â‚‚,áµ¢ O' 
            âˆ
            where open EqReasoning ğ•â‚‚â‚›

    prfO : (Î“â‚ƒ,â‚’ V) â‰ˆáµ¥,â‚‚ (Î“â‚‚,â‚’ V')
    prfO = Î“â‚‚,â‚’-cong Vâ‰ˆV'  


Sâ‚ƒâ‰ˆSâ‚‚-maintained-iter : âˆ€ (S3 : Î“â‚ƒ-State) (S2 : Î“â‚‚-State) k â†’ Sâ‚ƒâ‰ˆSâ‚‚ S3 S2 â†’ Î“â‚ƒ-invariant S3 â†’ Sâ‚ƒâ‰ˆSâ‚‚ ((Î“â‚ƒ ^ k) S3) ((Î“â‚‚ ^ k) S2)
Sâ‚ƒâ‰ˆSâ‚‚-maintained-iter S3 S2 zero eq inv = eq 
Sâ‚ƒâ‰ˆSâ‚‚-maintained-iter S3 S2 (suc k) eq inv =
   Sâ‚ƒâ‰ˆSâ‚‚-maintained ((Î“â‚ƒ ^ k) S3) ((Î“â‚‚ ^ k) S2) (Sâ‚ƒâ‰ˆSâ‚‚-maintained-iter S3 S2 k eq inv)  (Î“â‚ƒ-invariant-maintained-iter S3 k inv) 

Sâ‚ƒâ‰ˆSâ‚‚-init : Sâ‚ƒâ‰ˆSâ‚‚ ((~ M) , Ã˜áµ¥,â‚‚ , Ã˜áµ¥,â‚‚ , (Ã˜áµ¥,â‚‚ , Ã˜áµ¥,â‚‚)) ((~ M) , Ã˜áµ¥,â‚‚ , Ã˜áµ¥,â‚‚)
Sâ‚ƒâ‰ˆSâ‚‚-init = â‰ˆáµ¥-refl , ( â‰ˆáµ¥,â‚‚-refl , â‰ˆáµ¥,â‚‚-refl )

Î“â‚‚,áµ¢Ã˜â‰ˆÃ˜ : Î“â‚‚,áµ¢ Ã˜áµ¥,â‚‚ â‰ˆáµ¥,â‚‚ Ã˜áµ¥,â‚‚
Î“â‚‚,áµ¢Ã˜â‰ˆÃ˜ i j = â†­-refl 

Ã˜âˆªÃ˜â‰ˆÃ˜ : (Ã˜áµ¥,â‚‚ âˆªáµ¥ Ã˜áµ¥,â‚‚) â‰ˆáµ¥,â‚‚ Ã˜áµ¥,â‚‚
Ã˜âˆªÃ˜â‰ˆÃ˜ i j = â†­-refl 

Ã˜-Ã˜â‰ˆÃ˜ : (Ã˜áµ¥,â‚‚ -áµ¥ Ã˜áµ¥,â‚‚) â‰ˆáµ¥,â‚‚ Ã˜áµ¥,â‚‚
Ã˜-Ã˜â‰ˆÃ˜ i j = â†­-refl 

init-invariant : Î“â‚ƒ-invariant ((~ M) , Ã˜áµ¥,â‚‚ , Ã˜áµ¥,â‚‚ , (Ã˜áµ¥,â‚‚ , Ã˜áµ¥,â‚‚))
init-invariant  = prf
  where
    prf : Î“â‚‚,áµ¢ Ã˜áµ¥,â‚‚ â‰ˆáµ¥,â‚‚ Î“â‚ƒ,áµ¢ Ã˜áµ¥,â‚‚  (Ã˜áµ¥,â‚‚ , Ã˜áµ¥,â‚‚)
    prf = â‰ˆáµ¥,â‚‚-refl
         
Sâ‚ƒâ‰ˆSâ‚‚-maintained-init : âˆ€ k â†’ Sâ‚ƒâ‰ˆSâ‚‚ ((Î“â‚ƒ ^ k) ((~ M) , Ã˜áµ¥,â‚‚ , Ã˜áµ¥,â‚‚ , (Ã˜áµ¥,â‚‚ , Ã˜áµ¥,â‚‚))) ((Î“â‚‚ ^ k) ((~ M) , Ã˜áµ¥,â‚‚ , Ã˜áµ¥,â‚‚))
Sâ‚ƒâ‰ˆSâ‚‚-maintained-init  k = Sâ‚ƒâ‰ˆSâ‚‚-maintained-iter ((~ M) , Ã˜áµ¥,â‚‚ , Ã˜áµ¥,â‚‚ , (Ã˜áµ¥,â‚‚ , Ã˜áµ¥,â‚‚)) ((~ M) , Ã˜áµ¥,â‚‚ , Ã˜áµ¥,â‚‚) k Sâ‚ƒâ‰ˆSâ‚‚-init init-invariant
